Fill in more proofs

src/Specific/X86/Exponent25519.v
@@ -8,8 +8,10 @@ Require Import Crypto.BoundedArithmetic.X86ToZLikeProofs.
 Require Import Crypto.BoundedArithmetic.Eta.
 Require Import Crypto.ModularArithmetic.BarrettReduction.ZBounded.
 Require Import Crypto.ModularArithmetic.ZBoundedZ.
+Require Import Crypto.Spec.ModularArithmetic.
 Require Import Crypto.Util.Tuple.
 Require Import Crypto.Util.LetIn.
+Require Import Crypto.Util.Tactics.
 Import NPeano.
 
 Local Notation modulusv := (2^252 + 27742317777372353535851937790883648493)%Z.
@@ -19,8 +21,7 @@ Local Notation eta3 x := (eta (fst x), snd x).
 Local Notation eta4 x := (eta3 (fst x), snd x).
 Local Notation eta4' x := (eta (fst x), eta (snd x)).
 
-Section x86.
-  Axiom admit : forall {T}, T.
+Section Z.
   Definition SRep := Z. (*tuple x86.W (256/n).*)
   Definition SRepEq : Relation_Definitions.relation SRep := Logic.eq.
   Local Instance SRepEquiv : RelationClasses.Equivalence SRepEq := _.
@@ -62,10 +63,10 @@ Section x86.
   Local Existing Instance x86_25519_Barrett.
   Local Existing Instance x86_25519_BarrettProofs.
   Declare Reduction srep := cbv [barrett_reduce_function_bundled barrett_reduce_function BarrettBundled.m BarrettBundled.b BarrettBundled.k BarrettBundled.offset BarrettBundled.μ' ZBounded.ConditionalSubtractModulus ZBounded.CarrySubSmall  ZBounded.Mod_SmallBound ZBounded.Mod_SmallBound ZBounded.Mul ZBounded.DivBy_SmallBound ZBounded.DivBy_SmallerBound  ZBounded.modulus_digits x86_25519_Barrett BarrettBundled.ops ZZLikeOps ZBounded.CarryAdd Z.pow2_mod].
-  Definition SRepDecModL' : Word.word (256 + 256) -> SRep
+  Definition SRepDecModL : Word.word (256 + 256) -> SRep
     := Eval srep in
         fun w => dlet w := (Z.of_N (Word.wordToN w)) in barrett_reduce_function_bundled w.
-  Local Arguments SRepDecModL' / _.
+  (*Local Arguments SRepDecModL' / _.
   Ltac change_values v :=
     match v with
     | context vv[2 * ?x]
@@ -101,24 +102,107 @@ Section x86.
     let v := (*change_values*) v' in
     unify v v';
       exact v.
-  Defined.
-  (* TODO(jadep):what's S2Rep? *)
-  (*Lemma SRepDecModL_Correct : forall w : Word.word (b + b), SRepEq (S2Rep (ModularArithmetic.F.of_nat l (Word.wordToNat w))) (SRepDecModL w).*)
+  Defined.*)
+  Check @sign_correct _ _ _ _ _ _ _ _ _ _ _ _ _ _ ed25519.
+  Check @verify_correct _ _ _ _ _ _ _ _ _ _ _ _ _ _ ed25519.
+  Definition S2Rep : ModularArithmetic.F.F l -> SRep := F.to_Z.
+  Lemma Z_of_nat_of_word_eq_Z_of_N_of_word
+    : forall (n : nat) (w : Word.word n), Z.of_nat (Word.wordToNat w) = Z.of_N (Word.wordToN w).
+  Admitted.
+  Lemma SRepDecModL_Correct : forall w : Word.word (b + b), SRepEq (S2Rep (ModularArithmetic.F.of_nat l (Word.wordToNat w))) (SRepDecModL w).
+  Proof.
+    intro w; change (SRepDecModL w) with (barrett_reduce_function_bundled (Z.of_N (Word.wordToN w))).
+    unfold SRepEq, S2Rep, b in *.
+    pose proof (barrett_reduce_correct_bundled (Z.of_N (Word.wordToN w))) as H.
+    simpl in H; destruct H as [H _].
+    { pose proof (Word.wordToNat_bound w).
+      rewrite Word.wordToN_nat, nat_N_Z.
+      rewrite WordUtil.pow2_id in H.
+      change (Z.pow_pos 2 506) with (2^(253 + 253))%Z.
+      apply inj_lt in H.
+      rewrite Z.pow_Zpow, Nat2Z.inj_add in H; simpl @Z.of_nat in *.
+      split; auto with zarith.
+      admit. (* impossible *) }
+    { simpl in *; rewrite H; clear H.
+      rewrite Z_of_nat_of_word_eq_Z_of_N_of_word; reflexivity. }
+  Admitted.
   Definition SRepAdd : SRep -> SRep -> SRep
     := Eval srep in fun x y => barrett_reduce_function_bundled (snd (ZBounded.CarryAdd x y)).
-  (*Lemma SRepAdd_Correct forall x y : ModularArithmetic.F.F l, SRepEq (S2Rep (ModularArithmetic.F.add x y)) (SRepAdd (S2Rep x) (S2Rep y))).*)
+  Lemma SRepAdd_Correct : forall x y : ModularArithmetic.F.F l, SRepEq (S2Rep (ModularArithmetic.F.add x y)) (SRepAdd (S2Rep x) (S2Rep y)).
+  Proof.
+    intros x y; change (SRepAdd ?x ?y) with (barrett_reduce_function_bundled (snd (ZBounded.CarryAdd x y))).
+    unfold SRepEq, S2Rep, b in *; simpl.
+    match goal with
+    | [ |- context[barrett_reduce_function_bundled ?x] ]
+      => pose proof (barrett_reduce_correct_bundled x) as H
+    end.
+    pose proof (ModularArithmeticTheorems.F.to_Z_range x).
+    pose proof (ModularArithmeticTheorems.F.to_Z_range y).
+    unfold l in *.
+    specialize_by auto using modulusv_pos.
+    assert (F.to_Z x + F.to_Z y < 2 * modulusv - 1) by omega.
+    assert (2 * modulusv - 1 <= 2 ^ (253 + 253)) by (vm_compute; clear; intuition congruence).
+    assert (2^(253 + 253) < 2^512) by (vm_compute; clear; intuition congruence).
+    assert (0 <= F.to_Z x + F.to_Z y < 2^512) by omega.
+    simpl in H; destruct H as [H _].
+    { change (Z.pow_pos 2 506) with (2^(253 + 253))%Z.
+      rewrite Z.pow2_mod_spec by omega; Z.rewrite_mod_small.
+      simpl in *; omega. }
+    { simpl in H |- *; rewrite H; clear H.
+      rewrite Z.pow2_mod_spec by omega; Z.rewrite_mod_small.
+      reflexivity. }
+  Qed.
   Global Instance SRepAdd_Proper : Proper (SRepEq ==> SRepEq ==> SRepEq) SRepAdd.
   Proof. unfold SRepEq; repeat intro; subst; reflexivity. Qed.
   Definition SRepMul : SRep -> SRep -> SRep
     := Eval srep in fun x y => barrett_reduce_function_bundled (ZBounded.Mul x y).
-  (*Lemma SRepMul_Correct : forall x y : ModularArithmetic.F.F l, SRepEq (S2Rep (ModularArithmetic.F.mul x y)) (SRepMul (S2Rep x) (S2Rep y)). *)
+  Lemma SRepMul_Correct : forall x y : ModularArithmetic.F.F l, SRepEq (S2Rep (ModularArithmetic.F.mul x y)) (SRepMul (S2Rep x) (S2Rep y)).
+  Proof.
+    intros x y; change (SRepMul ?x ?y) with (barrett_reduce_function_bundled (ZBounded.Mul x y)).
+    unfold SRepEq, S2Rep, b in *; simpl.
+    match goal with
+    | [ |- context[barrett_reduce_function_bundled ?x] ]
+      => pose proof (barrett_reduce_correct_bundled x) as H
+    end.
+    pose proof (ModularArithmeticTheorems.F.to_Z_range x).
+    pose proof (ModularArithmeticTheorems.F.to_Z_range y).
+    unfold l in *.
+    specialize_by auto using modulusv_pos.
+    assert (0 <= F.to_Z x * F.to_Z y < modulusv * modulusv) by nia.
+    assert (modulusv * modulusv <= 2 ^ (253 + 253)) by (vm_compute; clear; intuition congruence).
+    assert (2^(253 + 253) < 2^512) by (vm_compute; clear; intuition congruence).
+    simpl in H; destruct H as [H _].
+    { change (Z.pow_pos 2 506) with (2^(253 + 253))%Z.
+      set (k := modulusv) in *; compute in k.
+      let v := (eval unfold k in k) in change v with k.
+      omega. }
+    { simpl in H |- *; rewrite H; clear H.
+      reflexivity. }
+  Qed.
   Global Instance SRepMul_Proper : Proper (SRepEq ==> SRepEq ==> SRepEq) SRepMul.
   Proof. unfold SRepEq; repeat intro; subst; reflexivity. Qed.
-  Definition SRepDecModLShort : Word.word (256 + 1) -> SRep
+  Definition SRepDecModLShort : Word.word (n + 1) -> SRep
     := Eval srep in
         fun w => dlet w := (Z.of_N (Word.wordToN w)) in barrett_reduce_function_bundled w.
-  (*Lemma SRepDecModLShort_Correct : forall w : Word.word (n + 1), SRepEq (S2Rep (ModularArithmetic.F.of_nat l (Word.wordToNat w))) (SRepDecModLShort w). *)
+  Lemma SRepDecModLShort_Correct : forall w : Word.word (n + 1), SRepEq (S2Rep (ModularArithmetic.F.of_nat l (Word.wordToNat w))) (SRepDecModLShort w).
+  Proof.
+    intro w; change (SRepDecModLShort w) with (barrett_reduce_function_bundled (Z.of_N (Word.wordToN w))).
+    unfold SRepEq, S2Rep, n, b in *.
+    pose proof (barrett_reduce_correct_bundled (Z.of_N (Word.wordToN w))) as H.
+    simpl in H; destruct H as [H _].
+    { pose proof (Word.wordToNat_bound w).
+      rewrite Word.wordToN_nat, nat_N_Z.
+      rewrite WordUtil.pow2_id in H.
+      change (Z.pow_pos 2 506) with (2^(253 + 253))%Z.
+      apply inj_lt in H.
+      rewrite Z.pow_Zpow, Nat2Z.inj_add in H; simpl @Z.of_nat in *.
+      split; auto with zarith.
+      assert (2^(254+1) < (2^(253+253))) by (vm_compute; reflexivity).
+      omega. }
+    { simpl in *; rewrite H; clear H.
+      rewrite Z_of_nat_of_word_eq_Z_of_N_of_word; reflexivity. }
+  Qed.
   Arguments Algebra.group : clear implicits.
   Check @sign_correct _ _ _ _ _ _ _ _ _ _ _ _ _ _ ed25519.
   Check @verify_correct _ _ _ _ _ _ _ _ _ _ _ _ _ _ ed25519.
-End x86.
+End Z.
